

Homework 3

Instructor: Lijun Zhang

Name: Renzhe Zhou, StudentId: 181220076

Notice

- The submission email is: **njuoptfall2019@163.com**.
- Please use the provided L^AT_EX file as a template. If you are not familiar with L^AT_EX, you can also use Word to generate a **PDF** file.

Problem 1: Equality Constrained Least-squares

Consider the equality constrained least-squares problem

$$\begin{aligned} & \text{minimize} && \frac{1}{2} \|Ax - b\|_2^2 \\ & \text{subject to} && Gx = h \end{aligned}$$

where $A \in \mathbf{R}^{m \times n}$ with **rank** $A = n$, and $G \in \mathbf{R}^{p \times n}$ with **rank** $G = p$.

- Derive the Lagrange dual problem with Lagrange multiplier vector v .
- Derive expressions for the primal solution x^* and the dual solution v^* .

Solution.

- The lagrange function is

$$L(x, v) = \frac{1}{2} \|Ax - b\|_2^2 + v^T(Gx - h) = \frac{1}{2} x^T A^T A x + (v^T G - b^T A)x + \frac{1}{2} b^T b - v^T h \quad (1)$$

Make $\nabla_x L(x, v) = A^T A x + G^T v - A^T b = 0$, we can get minimizer $x = (A^T A)^{-1}(A^T b - G^T v)$. So the dual function is

$$g(v) = \inf_x L(x, v) = -\frac{1}{2} (G^T v - A^T b)^T (A^T A)^{-1} (G^T v - A^T b) + \frac{1}{2} b^T b - v^T h \quad (2)$$

So the lagrange dual problem is

$$\text{maximize} \quad -\frac{1}{2} (G^T v - A^T b)^T (A^T A)^{-1} (G^T v - A^T b) + \frac{1}{2} b^T b - v^T h$$

- From KKT conditions we can get $\nabla L(x^*, v^*) = A^T A x^* + G^T v^* - A^T b = 0$ and $Gx^* = h$. Make $x^* = (A^T A)^{-1}(A^T b - G^T v^*)$ into $Gx^* = h$ we can get

$$v^* = (G(A^T A)^{-1} G^T)^{-1} (G(A^T A)^{-1} A^T b - h) \quad (3)$$

Therefore we get

$$x^* = (A^T A)^{-1} (A^T b - G^T (G(A^T A)^{-1} G^T)^{-1} (G(A^T A)^{-1} A^T b - h)) \quad (4)$$

Done. □

Problem 2: Support Vector Machines

Consider the following optimization problem

$$\text{minimize} \quad \sum_{i=1}^n \max(0, 1 - y_i(w^T x_i + b)) + \frac{\lambda}{2} \|w\|_2^2$$

where $x_i \in \mathbf{R}^d$, $y_i \in \mathbf{R}$, $i = 1, \dots, n$ are given, and $w \in \mathbf{R}^d$, $b \in \mathbf{R}$ are the variables.

a) Derive an equivalent problem by introducing new variables u_i , $i = 1, \dots, n$ and equality constraints

$$u_i = y_i(w^T x_i + b), i = 1, \dots, n.$$

b) Derive the Lagrange dual problem of the above equivalent problem.

c) Give the Karush-Kuhn-Tucker conditions.

Hint: Let $\ell(x) = \max(0, 1 - x)$. Its conjugate function $\ell^(y) = \sup_x (yx - \ell(x)) = \begin{cases} y, & -1 \leq y \leq 0 \\ \infty, & \text{otherwise} \end{cases}$*

Solution.

a) The problem is:

$$\begin{aligned} &\text{minimize} \quad \sum_{i=1}^n \max(0, 1 - u_i) + \frac{\lambda}{2} \|w\|_2^2 \\ &\text{subject to} \quad u_i = y_i(w^T x_i + b), i = 1, \dots, n. \end{aligned} \quad (5)$$

b) The Lagrange function is

$$L(w, b, u_1, \dots, u_n, v_1, \dots, v_n) = \sum_{i=1}^n \max(0, 1 - u_i) + \frac{\lambda}{2} \|w\|_2^2 + \sum_{i=1}^n v_i(u_i - y_i(w^T x_i + b)) \quad (6)$$

To get the dual function, minimize w , b and u_i . Minimize w , we have $\frac{\partial L}{\partial w} = \lambda w + \sum_{i=1}^n (-v_i y_i x_i) = 0$. So $w^* = \frac{1}{\lambda} \sum_{i=1}^n v_i y_i x_i$. Minimize b , we have $\frac{\partial L}{\partial b} = \sum_{i=1}^n (-v_i y_i) = 0$, if not, the minimum could be $-\infty$. And $\sum_{i=1}^n v_i y_i x_i^T (\sum_{j=1}^n v_j y_j x_j) = \sum_{i=1}^n v_i y_i (\sum_{j=1}^n v_j y_j x_i^T x_j)$. Therefore, in that case, let $l(u_i) = \max(0, 1 - u_i)$, we have:

$$\begin{aligned} g(v_1, \dots, v_n) &= \frac{1}{2|\lambda|} \left\| \sum_{i=1}^n v_i y_i x_i \right\|_2^2 - \frac{1}{\lambda} \sum_{i=1}^n v_i y_i \left(\sum_{j=1}^n v_j y_j x_i^T x_j \right) + \inf_{u_i} \left(\sum_{i=1}^n \max(0, 1 - u_i) + v_i u_i \right) \\ &= \frac{1}{2|\lambda|} \left\| \sum_{i=1}^n v_i y_i x_i \right\|_2^2 - \frac{1}{\lambda} \sum_{i=1}^n v_i y_i \left(\sum_{j=1}^n v_j y_j x_i^T x_j \right) - \sum_{i=1}^n l^*(-v_i) \end{aligned} \quad (7)$$

To maximize it, we must have $0 \leq v_i \leq 1$. So the Lagrange dual problem is:

$$\begin{aligned} &\text{maximize} \quad \frac{1}{2|\lambda|} \left\| \sum_{i=1}^n v_i y_i x_i \right\|_2^2 - \frac{1}{\lambda} \sum_{i=1}^n v_i y_i \left(\sum_{j=1}^n v_j y_j x_i^T x_j \right) + \sum_{i=1}^n v_i \\ &\text{subject to} \quad \sum_{i=1}^n v_i y_i = 0, \quad 0 \leq v_i \leq 1, i = 1, \dots, n. \end{aligned} \quad (8)$$

c) The KKT conditions are:

$$\begin{aligned} w^* &= \frac{1}{\lambda} \sum_{i=1}^n v_i^* y_i x_i \\ \sum_{i=1}^n v_i^* y_i &= 0 \\ u_i^* &= y_i(w^{*T} x_i + b^*), i = 1, \dots, n. \end{aligned} \quad (9)$$

Done.

□

Problem 3: Euclidean Projection onto the Simplex

Consider the following optimization problem

$$\begin{aligned} & \text{minimize} && \frac{1}{2} \|y - x\|_2^2 \\ & \text{subject to} && \mathbf{1}^T y = r \\ & && y \succeq 0 \end{aligned}$$

where $r > 0$, $x \in \mathbb{R}^n$ is given, and $y \in \mathbb{R}^n$ is the variable. Give an algorithm to solve this problem and prove the correctness of your algorithm.

Hint: Derive the Lagrangian of this problem and apply the Karush-Kuhn-Tucker conditions. If you need more hints, please read the following paper [1]

Solution.

1. Algorithm:

Input: $x \in \mathbb{R}^n$

Sort x into $u: u_1 \geq u_2 \geq \dots \geq u_n$

Find $\rho = \max\{1 \leq j \leq n : u_j + \frac{1}{j}(r - \sum_{i=1}^j u_i) > 0\}$

Define $\lambda = \frac{1}{\rho}(r - \sum_{i=1}^{\rho} u_i)$

Output: y s.t. $y_i = \max\{x_i + \lambda, 0\}, i = 1, \dots, n$.

2. Proof:

The lagrange function of this problem is (λ and v is the equality and inequality Lagrange multipliers respectively)

$$L(y, \lambda, v) = \frac{1}{2} \|y - x\|_2^2 - \lambda(\mathbf{1}^T y - r) - v^T y \quad (10)$$

Assume the optimal solution y then the KKT conditions are following:

$$y_i - x_i - \lambda - v_i = 0, \quad y_i \geq 0, v_i \geq 0, \quad v_i y_i = 0, \quad \sum_{i=1}^n y_i = r \quad (11)$$

From $v_i y_i = 0$ we have

$$\begin{aligned} & \text{if } y_i > 0 : v_i = 0, y_i = x_i + \lambda > 0 \\ & \text{if } y_i = 0 : v_i \geq 0, y_i = x_i + \lambda + v_i = 0, \text{ which is } x_i + \lambda = -v_i < 0 \end{aligned} \quad (12)$$

So the components of the optimal solution y that are zeros correspond to the smaller components of x . Assume the components of x are sorted and y uses the same ordering:

$$\begin{aligned} x_1 &\geq \dots \geq x_{\rho} \geq x_{\rho+1} \geq \dots \geq x_n \\ y_1 &\geq \dots \geq y_{\rho} \geq y_{\rho+1} = \dots = y_n = 0 \end{aligned} \quad (13)$$

where ρ is the number of positive components of y . So from $\sum_{i=1}^n y_i = r$ we have

$$\sum_{i=1}^n y_i = \sum_{i=1}^{\rho} y_i = \sum_{i=1}^{\rho} (x_i + \lambda) = r \quad (14)$$

Which implies $\lambda = \frac{1}{\rho}(r - \sum_{i=1}^{\rho} x_i)$. So if we can compute ρ then we know λ and then we know the optimal solution y because $y_i = x_i + \lambda$ if $x_i + \lambda > 0$ else $y_i = 0$.

Therefore, we are going to prove $\rho = \max\{1 \leq j \leq n : x_j + \frac{1}{j}(r - \sum_{i=1}^j x_i) > 0\}$.

We have $\lambda \rho = r - \sum_{i=1}^{\rho} x_i$, we are going to show that $x_j + \frac{1}{j}(r - \sum_{i=1}^j x_i) > 0$ for $j \leq \rho$ and $x_j + \frac{1}{j}(r - \sum_{i=1}^j x_i) \leq 0$ for $j > \rho$.

1) $j = \rho$, we have $x_{\rho} + \frac{1}{\rho}(r - \sum_{i=1}^{\rho} x_i) = x_{\rho} + \lambda = y_{\rho} > 0$

2) $j < \rho$, we have

$$\begin{aligned} x_j + \frac{1}{j}(r - \sum_{i=1}^j x_i) &= \frac{1}{j}(jx_j + r - \sum_{i=1}^j x_i) = \frac{1}{j}(jx_j + \sum_{i=j+1}^{\rho} x_i + r - \sum_{i=1}^{\rho} x_i) \\ &= \frac{1}{j}(jx_j + \sum_{i=j+1}^{\rho} x_i + \rho\lambda + j\lambda - j\lambda) = \frac{1}{j}(j(x_j + \lambda) + \sum_{i=j+1}^{\rho} (x_i + \lambda)) \end{aligned} \quad (15)$$

Because $x_i + \lambda > 0$ for $i = j, \dots, \rho$, so $x_j + \frac{1}{j}(r - \sum_{i=1}^j x_i) > 0$.

3) $j > \rho$, we have

$$\begin{aligned} x_j + \frac{1}{j}(r - \sum_{i=1}^j x_i) &= \frac{1}{j}(jx_j + r - \sum_{i=1}^j x_i) = \frac{1}{j}(jx_j + r - \sum_{i=1}^{\rho} x_i - \sum_{i=\rho+1}^j x_i) \\ &= \frac{1}{j}(jx_j + \rho\lambda - \sum_{i=\rho+1}^j x_i + \rho x_j - \rho x_j) = \frac{1}{j}(\rho(x_j + \lambda) + \sum_{i=\rho+1}^j (x_j - x_i)) \end{aligned} \quad (16)$$

Because $x_j + \lambda \leq 0$ for $j > \rho$ and $x_j - x_i \leq 0$ for $j \geq i$ since x is sorted, we have $x_j + \frac{1}{j}(r - \sum_{i=1}^j x_i) < 0$.

Therefore, $\rho = \max\{1 \leq j \leq n : x_j + \frac{1}{j}(r - \sum_{i=1}^j x_i) > 0\}$ correctly denotes the number of positive components of y , and we can know λ and we get the optimal solution y by computing $y_i = \max\{x_i + \lambda, 0\}$ since x is given.

Above all, the Algorithm can correctly give the optimal solution of the problem.

Done.

□

Problem 4: Optimality Conditions

Consider the problem

$$\begin{aligned} &\text{minimize} && \text{tr}(2X) - \log \det(3X) \\ &\text{subject to} && 2Xs = y \end{aligned}$$

with variable $X \in \mathbf{S}^n$ and domain \mathbf{S}_{++}^n . Here, $y \in \mathbf{R}^n$ and $s \in \mathbf{R}^n$ are given, with $s^T y = 1$.

a) Give the Lagrange and then derive the Karush-Kuhn-Tucker conditions.

b) Verify that the optimal solution is given by

$$X^* = \frac{1}{2} \left(I + yy^T - \frac{ss^T}{s^T s} \right).$$

Solution.

a) The lagrange function is $L(X, v) = \text{tr}(2X) - \log \det(3X) - v^T(2Xs - y)$. And $\nabla_X L(X, v) = 2I - X^{-1} + (vs^T + sv^T)$. So the KKT conditions are:

$$X^* \succ 0, \quad 2X^*s = y, \quad 2I - X^{*-1} + (vs^T + sv^T) = 0 \quad (17)$$

b) We have

$$s = \frac{1}{2}X^{*-1}y = (I + \frac{1}{2}(vs^T + sv^T))y = y + \frac{1}{2}(vs^T y + sv^T y) = y + \frac{1}{2}(v + v^T y s) \quad (18)$$

So

$$y^T s = 1 = y^T(y + \frac{1}{2}(v + v^T y s)) = y^T y + \frac{1}{2}(y^T v + y^T v^T y s) = y^T y + \frac{1}{2}(v^T y + (v^T y)y^T s) = y^T y + v^T y \quad (19)$$

Take $v^T y = 1 - y^T y$ into $s = y + \frac{1}{2}(v + (v^T y)s)$ then we have

$$v = (1 + y^T y)s - 2y \quad (20)$$

Therefore,

$$\begin{aligned} X^{*-1} &= 2I + ((1 + y^T y)s - 2y)s^T + s((1 + y^T y)s^T - 2y^T) \\ &= 2I + 2(1 + y^T y)ss^T - 2ys^T - 2sy^T \end{aligned} \quad (21)$$

Multiply it with the condition given above:

$$\begin{aligned}
& [2I + 2(1 + y^T y)ss^T - 2ys^T - 2sy^T][\frac{1}{2}(I + yy^T - \frac{ss^T}{s^T s})] \\
&= (I + yy^T - \frac{ss^T}{s^T s} + (1 + y^T y)(ss^T + sy^T - ss^T) - (ys^T + yy^T - ys^T) - (sy^T + (y^T y)sy^T - \frac{ss^T}{s^T s})) \quad (22) \\
&= I + yy^T - yy^T - (\frac{ss^T}{s^T s}) + (\frac{ss^T}{s^T s}) + (1 + y^T y)sy^T - (1 + y^T y)sy^T \\
&= I
\end{aligned}$$

Therefore, the inverse matrix of $2I + 2(1 + y^T y)ss^T - 2ys^T - 2sy^T$ is $\frac{1}{2}(I + yy^T - \frac{ss^T}{s^T s})$

So $X^* = (X^{*-1})^{-1} = \frac{1}{2}(I + yy^T - \frac{ss^T}{s^T s})$.

Done.

□

References

- [1] Weiran Wang, and Miguel Á. Carreira-Peroiñán. Projection onto the probability simplex: An efficient algorithm with a simple proof, and an application. *arXiv:1309.1541*, 2013.